steel/Veritas.Steel.PRFSetHash.fsti
@@ -1,0 +1,46 @@
+module Veritas.Steel.PRFSetHash
+
+open Steel.Memory
+open Steel.Effect.Atomic
+open Steel.Effect
+open Steel.Reference
+open Steel.Array
+open FStar.Ghost
+module U16 = FStar.UInt16
+module U32 = FStar.UInt32
+module U64 = FStar.UInt64
+
+module T = Veritas.Formats.Types
+open Veritas.Steel.VerifierModel
+open Veritas.ThreadStateModel
+val prf_set_hash : Type0
+
+// AF: Internally, should probably be implemented with a ghost reference to the model_hash
+// The selector would then fetch the value in the ghost state
+// The reason why we would need a ghost state is that the "spec" contains strictly more
+// information than the concrete value. So we cannot reconstruct it out of just the concrete state
+val prf_set_hash_sl (_:prf_set_hash) : slprop u#1
+val prf_set_hash_sel (r:prf_set_hash) : selector (model_hash) (prf_set_hash_sl r)
+
+[@@__steel_reduce__]
+noextract
+let prf_set_hash_inv' (r:prf_set_hash) : vprop' =
+  { hp = prf_set_hash_sl r;
+    t = model_hash;
+    sel = prf_set_hash_sel r}
+
+unfold
+let prf_set_hash_inv (r:prf_set_hash) : vprop = VUnit (prf_set_hash_inv' r)
+
+[@@ __steel_reduce__]
+let v_hash (#p:vprop) (r:prf_set_hash)
+  (h:rmem p{FStar.Tactics.with_tactic selector_tactic (can_be_split p (prf_set_hash_inv r) /\ True)})
+  : GTot model_hash
+  = h (prf_set_hash_inv r)
+
+val prf_update_hash (p:prf_set_hash) (r:T.record) (t:T.timestamp) (thread_id:T.thread_id)
+  : Steel unit
+    (prf_set_hash_inv p)
+    (fun _ -> prf_set_hash_inv p)
+    (requires fun _ -> True)
+    (ensures fun h0 _ h1 -> v_hash p h1 == model_update_hash (v_hash p h0) r t thread_id)
